coq/CAMP/Lang/CAMP.v
@@ -14,55 +14,88 @@
  * limitations under the License.
  *)
 
+(** CAMP is a small calculus for pattern matching. Its purpose is to
+  capture the semantics of rules languages that rely on the ability to
+  recover from match failure. *)
+
+(** Two distinct evaluation functions for CAMP are defined. The first
+  is a standard evaluation function and serves as semantic
+  definition. The second is equivalent but maintains a trace of the
+  evaluation for debugging purposes. *)
+  
+(** Summary:
+- Language: CAMP (Calculus for Aggregating Matching Patterns)
+- Based on: "A Pattern Calculus for Rule Languages:
+  Expressiveness, Compilation, and Mechanization" Avraham
+  Shinnar, Jérôme Siméon, and Martin Hirzel. ECOOP'2015.
+- URL: http://drops.dagstuhl.de/opus/volltexte/2015/5237/
+- Languages translating to CAMP: TechRule, DesignRule, CAMPRule, cNNRC
+- Languages translating from CAMP: NRA, cNRAEnv, NRAEnv
+*)
+  
 Section CAMP.
 
   Require Import String.
   Require Import List.
   Require Import EquivDec.
   Require Import Morphisms.
-
   Require Import BasicRuntime.
+  Require Import CAMPUtil.
+  
+  Local Open Scope string.
 
   Context {fruntime:foreign_runtime}.
 
+  (** * Abstract Syntax *)
+
+  (** CAMP patterns are pure expressions. They match against a current
+  value in the context of an environment. The environment has a
+  globale component which is static, and a local component which can
+  be modified in the course of evaluation. *)
+
+  (** Operations include: pmap, a functional map which skips match
+  failure; passert, which turns match failure into a terminal failure,
+  and porElse which allows to continue to a new pattern in case of
+  match failure. *)
+
+  (** Compared to the published material, three new operators are
+  added: pgetConstant which accesses the global environment, pleft and
+  pright which support pattern matching against choice values. *)
+  
+  Inductive camp : Set :=
+  | pconst : data -> camp                  (**r Constant value *)
+  | punop : unaryOp -> camp -> camp        (**r Unary operators *)
+  | pbinop : binOp -> camp -> camp -> camp (**r Binary operators *)
+  | pmap : camp -> camp                    (**r Functional map *)
+  | passert : camp -> camp                 (**r Assert pattern-matching success *)
+  | porElse : camp -> camp -> camp         (**r Recover from failure *)
+  | pit : camp                             (**r Current value being matched *)
+  | pletIt : camp -> camp -> camp          (**r Set the current value *)
+  | pgetConstant : string -> camp          (**r Access to a global variable *)
+  | penv : camp                            (**r Current environment *)
+  | pletEnv : camp -> camp -> camp         (**r Add bindings to the environment *)
+  | pleft : camp                           (**r Matches if the value is a left choice *)
+  | pright : camp.                         (**r Matches if the value is a right choice *)
+
   (* begin hide *)
-  Definition Var := nat.
+  Tactic Notation "camp_cases" tactic(first) ident(c) :=
+    first;
+    [ Case_aux c "pconst"%string
+    | Case_aux c "punop"%string
+    | Case_aux c "pbinop"%string
+    | Case_aux c "pmap"%string
+    | Case_aux c "passert"%string
+    | Case_aux c "porElse"%string
+    | Case_aux c "pit"%string
+    | Case_aux c "pletIt"%string
+    | Case_aux c "pgetConstant"%string
+    | Case_aux c "penv"%string
+    | Case_aux c "pletEnv"%string
+    | Case_aux c "pleft"%string
+    | Case_aux c "pright"%string].
   (* end hide *)
 
-  (** Patterns in CAMP *)
-  Inductive camp : Set :=
-  | pconst : data -> camp   (* This allows the empty list and empty record to be created *)
-  | punop : unaryOp -> camp -> camp (* this does need the first pattern argument, but providing it is more uniform with respect to pbinop *)
-  | pbinop : binOp -> camp -> camp -> camp
-  | pmap : camp -> camp
-(*| pgroupBy : camp -> camp *)
-  | passert : camp -> camp (* converts (dbool true) to [], and everything else to match failure *)
-  | porElse : camp -> camp -> camp (* if the first pattern fails, try the second pattern *)
-  | pit : camp
-  | pletIt : camp -> camp -> camp
-  | pgetconstant : string -> camp
-  | penv : camp
-    (* Run the first pattern, which must return a record of new bindings. This is merged with the current bindings, and used to run the second pattern *)
-  | pletEnv : camp -> camp -> camp
-  | pleft : camp
-  | pright : camp.
-
-  Tactic Notation "camp_cases" tactic(first) ident(c) :=
-  first;
-  [ Case_aux c "pconst"%string
-  | Case_aux c "punop"%string
-  | Case_aux c "pbinop"%string
-  | Case_aux c "pmap"%string
-(*| Case_aux c "pgroupBy"%string *)
-  | Case_aux c "passert"%string
-  | Case_aux c "porElse"%string
-  | Case_aux c "pit"%string
-  | Case_aux c "pletIt"%string
-  | Case_aux c "pgetconstant"%string
-  | Case_aux c "penv"%string
-  | Case_aux c "pletEnv"%string
-  | Case_aux c "pleft"%string
-  | Case_aux c "pright"%string].
+  (** Equality between two CAMP patterns is decidable. *)
   
   Global Instance camp_eqdec : EqDec camp eq.
   Proof.
@@ -74,38 +107,107 @@ Section CAMP.
     apply string_dec.
   Qed.
 
-  Local Open Scope string.
+  (** * Evaluation Semantics *)
+  
+  (** Evaluation takes a camp pattern, a global environment, a local
+    environment and a current value. It returns a presult which can be
+    either a successful evaluation holding a value, a match failure,
+    or a terminal failure. *)
 
+  (** The external context for evaluation includes a brand relation,
+    and a global environment. *)
+  
+  Section Evaluation.
+    Context (h:brand_relation_t).
+    Context (constant_env:bindings).
+
+    Fixpoint camp_eval (p:camp) (bind:bindings) (d:data) : presult data
+      := match p with
+         | pconst d' => Success (normalize_data h d')
+         | punop op p₁ => bindpr (camp_eval p₁ bind d)
+                                 (fun d' => (op2tpr (fun_of_unaryop h op d')))
+         | pbinop op p₁ p₂ => 
+           bindpr (camp_eval p₁ bind d)
+                  (fun d'₁ => 
+                     bindpr (camp_eval p₂ bind d)
+                            (fun d'₂ =>  (op2tpr (fun_of_binop h op d'₁ d'₂))))
+         | pmap p₁ =>
+           match d with
+           | dcoll l => liftpr dcoll (gather_successes (map (camp_eval p₁ bind) l))
+           | _ => TerminalError
+           end
+         | passert p₁ =>     
+           bindpr (camp_eval p₁ bind d)
+                  (fun d' => match d' with
+                             | dbool true => Success (drec nil)
+                             | dbool false => RecoverableError
+                             | _ => TerminalError 
+                             end)
+         | porElse p₁ p₂ =>
+           match camp_eval p₁ bind d with
+           | TerminalError => TerminalError
+           | RecoverableError => camp_eval p₂ bind d
+           | Success x => Success x
+           end
+         | pit => Success d
+         | pletIt p₁ p₂ =>
+           bindpr (camp_eval p₁ bind d) (camp_eval p₂ bind)
+         | pgetConstant s => op2tpr (edot constant_env s)
+         | penv => Success (drec bind)
+         | pletEnv p₁ p₂ =>
+           bindpr (camp_eval p₁ bind d)
+                  (fun rd'₁ => match rd'₁ with
+                               | drec d'₁ => match merge_bindings bind d'₁ with
+                                             | Some bind' => camp_eval p₂ bind' d
+                                             | None => RecoverableError
+                                             end
+                               | _ => TerminalError 
+                               end)
+         | pleft =>
+           match d with
+           | dleft d' => Success d'
+           | dright _ => RecoverableError 
+           | _ => TerminalError 
+           end
+         | pright =>
+           match d with
+           | dright d' => Success d'
+           | dleft _ => RecoverableError
+           | _ => TerminalError 
+           end
+         end.
+
+  End Evaluation.
+
+  (** * Pretty Printing *)
+
+  (** Evaluation traces rely on printing support for CAMP's abstract syntax. *)
+    
   Global Instance ToString_camp : ToString camp
     := { toString :=
            fix toStringp (p:camp) : string :=
              match p with
-               | pconst d => "(pconst " ++ toString d ++ ")"
-               | punop u p1 => "(punop " ++ toString u ++ " " ++ toStringp p1 ++ ")"
-               | pbinop b p1 p2 => "(pbinop " ++ toString b ++ " " ++ toStringp p1++ " " ++ toStringp p2 ++ ")"
-               | pmap p1 => "(pmap " ++ toStringp p1 ++ ")"
-               | passert p1 => "(passert " ++ toStringp p1 ++ ")"
-               | porElse p1 p2 => "(porElse " ++ toStringp p1++ " " ++ toStringp p2 ++ ")"
-               | pit  => "pit"
-               | pletIt p1 p2 => "(pletIt " ++ toStringp p1++ " " ++ toStringp p2 ++ ")"
-               | pgetconstant s => "(pgetconstant " ++ s ++ ")"
-               | penv => "penv"
-               | pletEnv p1 p2 => "(pletEnv " ++ toStringp p1++ " " ++ toStringp p2 ++ ")"
-               | pleft => "pleft"
-               | pright => "pright"
+             | pconst d => "(pconst " ++ toString d ++ ")"
+             | punop u p1 => "(punop " ++ toString u ++ " " ++ toStringp p1 ++ ")"
+             | pbinop b p1 p2 => "(pbinop " ++ toString b ++ " " ++ toStringp p1++ " " ++ toStringp p2 ++ ")"
+             | pmap p1 => "(pmap " ++ toStringp p1 ++ ")"
+             | passert p1 => "(passert " ++ toStringp p1 ++ ")"
+             | porElse p1 p2 => "(porElse " ++ toStringp p1++ " " ++ toStringp p2 ++ ")"
+             | pit  => "pit"
+             | pletIt p1 p2 => "(pletIt " ++ toStringp p1++ " " ++ toStringp p2 ++ ")"
+             | pgetConstant s => "(pgetConstant " ++ s ++ ")"
+             | penv => "penv"
+             | pletEnv p1 p2 => "(pletEnv " ++ toStringp p1++ " " ++ toStringp p2 ++ ")"
+             | pleft => "pleft"
+             | pright => "pright"
              end
        }.
-
-  (* If we were reasoning about this formally, we would want to use a proper
-     one-hole context.  Since we are not, a trail of choices suffices *)
-  Definition camp_src_path
-    := list nat.
-
+  
   Fixpoint toString_camp_with_path (p:camp) (loc:camp_src_path) :=
     match loc with
-      | nil => bracketString "<<<"  (toString p) ">>>"
-      | pos::loc' =>
-        match p with
+    | nil => bracketString "<<<"  (toString p) ">>>"
+    | pos::loc' =>
+      match p with
       | pconst d => "(pconst " ++ toString d ++ ")"
       | punop u p1 => "(punop " ++ toString u ++ " " ++
                                 toString_camp_with_path p1 loc' ++ ")"
@@ -121,599 +223,307 @@ Section CAMP.
       | pmap p1 => "(pmap " ++ toString_camp_with_path p1 loc' ++ ")"
       | passert p1 => "(passert " ++ toString_camp_with_path p1 loc' ++ ")"
       | porElse p1 p2 => "(porElse " ++
-                            (if pos == 0
-                             then toString_camp_with_path p1 loc'
-                             else toString p1)
-                            ++ " " ++
-                            (if pos == 1
-                             then toString_camp_with_path p2 loc'
-                             else toString p2) ++ ")"
-
+                                     (if pos == 0
+                                      then toString_camp_with_path p1 loc'
+                                      else toString p1)
+                                     ++ " " ++
+                                     (if pos == 1
+                                      then toString_camp_with_path p2 loc'
+                                      else toString p2) ++ ")"
       | pit  => "pit"
       | pletIt p1 p2 => "(pletIt " ++
-                            (if pos == 0
-                             then toString_camp_with_path p1 loc'
-                             else toString p1)
-                            ++ " " ++
-                            (if pos == 1
-                             then toString_camp_with_path p2 loc'
-                             else toString p2) ++ ")"
-      | pgetconstant s => "(pgetconstant " ++ s ++ ")"
+                                   (if pos == 0
+                                    then toString_camp_with_path p1 loc'
+                                    else toString p1)
+                                   ++ " " ++
+                                   (if pos == 1
+                                    then toString_camp_with_path p2 loc'
+                                    else toString p2) ++ ")"
+      | pgetConstant s => "(pgetConstant " ++ s ++ ")"
       | penv => "penv"
       | pletEnv p1 p2 => "(pletEnv " ++ 
-                            (if pos == 0
-                             then toString_camp_with_path p1 loc'
-                             else toString p1)
-                            ++ " " ++
-                            (if pos == 1
-                             then toString_camp_with_path p2 loc'
-                             else toString p2) ++ ")"
-
+                                     (if pos == 0
+                                      then toString_camp_with_path p1 loc'
+                                      else toString p1)
+                                     ++ " " ++
+                                     (if pos == 1
+                                      then toString_camp_with_path p2 loc'
+                                      else toString p2) ++ ")"
+                                     
       | pleft => "pleft"
       | pright => "pright"
-    end
+      end
     end.
-
-  Section eval.
-  (** Evaluating a pattern returns a presult.  The error strings are for debugging purposes *)
-
-  Inductive presult A :=
-  | TerminalError : presult A
-  | RecoverableError : presult A
-  | Success (res:A) : presult A.
-
-  (* begin hide *)
-  Arguments TerminalError {A}.
-  Arguments RecoverableError {A}.
-  Arguments Success {A} res.
-  (* end hide *)
-  
-  Global Instance print_presult {A} {tos:ToString A} : ToString (presult A)
-    := { toString :=
-           fun pr =>
-             match pr with
-               | TerminalError => "TerminalError (for more info, use debug mode)"
-               | RecoverableError => "RecoverableError (for more info, use debug mode)"
-               | Success res => "Success: " ++ toString res
-             end
-       }.
-  
-  Global Instance presult_eqdec {A} {dec:EqDec A eq} :
-    EqDec (presult A) eq.
-  Proof.
-    red; unfold equiv, complement.
-    destruct x; destruct y; simpl;
-    try solve [right; inversion 1]; eauto 2.
-    destruct (res == res0); unfold equiv, complement in *;
-    [left | right; inversion 1]; congruence.
-  Defined.
-  
-
-  (** Useful lifting functions used in the evaluation of patterns. Used to handle the various possible presults *)
-  Definition liftpr {A B:Type} (f:A->B) (pr:presult A) : presult B
-    := match pr with
-       | TerminalError => TerminalError
-       | RecoverableError => RecoverableError
-       | Success a => Success (f a)
-       end.
-
-  Definition bindpr {A B:Type} (pr:presult A) (f:A->presult B) : presult B
-    := match pr with
-       | TerminalError => TerminalError 
-       | RecoverableError => RecoverableError
-       | Success a => (f a)
-       end.
-
-  Lemma liftpr_bindpr {A B:Type} (f:A->B) pr :
-    liftpr f pr = bindpr pr (fun x => Success (f x)).
-  Proof.
-    destruct pr; simpl; trivial.
-  Qed.
-
-  Fixpoint gather_successes {A:Type} (os:list (presult A)) : presult (list A)
-    := match os with
-       | nil => Success nil
-       | (TerminalError)::xs => TerminalError 
-       | (RecoverableError)::xs => gather_successes xs
-       | (Success a)::xs => liftpr (cons a) (gather_successes xs)
-       end.
-
-  Fixpoint enforce_successes {A:Type} (os:list (presult A)) : presult (list A)
-    := match os with
-       | nil => Success nil
-       | (TerminalError)::xs => TerminalError
-       | (RecoverableError)::xs => RecoverableError
-       | (Success a)::xs => liftpr (cons a) (gather_successes xs)
-       end.
-
-  Definition op2tpr {A:Type} (o:option A) : presult A
-    := match o with
-       | None => TerminalError
-       | Some x => Success x
-       end.
-
-  (* begin hide *)
-  Definition op2rpr {A:Type} (o:option A) : presult A
-    := match o with
-       | None => RecoverableError
-       | Some x => Success x
-       end.
-
-  Definition pr2op (o:presult data) : option data
-    := match o with
-       | RecoverableError => None
-       | TerminalError => Some dunit
-       | Success x => Some x
-       end.
-  
-  (* end hide *)
-
-  (** Semantics of CAMP pattern, returning a presult *)
-  Context (h:brand_relation_t).
-  Context (constant_env:bindings).
-        
-  Fixpoint interp (p:camp) (bind:bindings) (d:data) : presult data
-    := match p with
-       | pconst d' => Success (normalize_data h d')
-       | punop op p₁ => bindpr (interp p₁ bind d)
-                               (fun d' => (op2tpr (fun_of_unaryop h op d')))
-       | pbinop op p₁ p₂ => 
-         bindpr (interp p₁ bind d)
-                (fun d'₁ => 
-                   bindpr (interp p₂ bind d)
-                          (fun d'₂ =>  (op2tpr (fun_of_binop h op d'₁ d'₂))))
-       | pmap p₁ =>
-         match d with
-         | dcoll l => liftpr dcoll (gather_successes (map (interp p₁ bind) l))
-         | _ => TerminalError
-
-         end
-(* Adds some unexpected complexity since the pattern used to calculate the key may return match failure.
-   How should we handle it? One option is to turn match failure into dunit, which possibly pushes part of the complexity
-   down to the algebra. Not sure what the other
-   options are ... - J
-       | pgroupBy p₁ =>
-         match d with
-         | dcoll l => op2tpr "groupBy failed"
-                             (lift dcoll
-                                   (group_by_nested_eval_kv (fun x => pr2op (interp p₁ bind x)) l))
-         | _ => TerminalError "pgroupBy evaluated when scrutinee is not a collection"
-         end *)
-       | passert p₁ =>     
-         bindpr (interp p₁ bind d)
-                (fun d' => match d' with
-                           | dbool true => Success (drec nil)
-                           | dbool false => RecoverableError
-                           | _ => TerminalError 
-                           end)
-       | porElse p₁ p₂ =>
-         match interp p₁ bind d with
-         | TerminalError => TerminalError
-         | RecoverableError => interp p₂ bind d
-         | Success x => Success x
-         end
-       | pit => Success d
-       | pletIt p₁ p₂ =>
-         bindpr (interp p₁ bind d) (interp p₂ bind)
-       | pgetconstant s => op2tpr (edot constant_env s)
-       | penv => Success (drec bind)
-       | pletEnv p₁ p₂ =>
-         bindpr (interp p₁ bind d)
-                (fun rd'₁ => match rd'₁ with
-                             | drec d'₁ => match merge_bindings bind d'₁ with
-                                           | Some bind' => interp p₂ bind' d
-                                           | None => RecoverableError
-                                           end
-                             | _ => TerminalError 
-                             end)
-       | pleft =>
-         match d with
-         | dleft d' => Success d'
-         | dright _ => RecoverableError 
-         | _ => TerminalError 
-         end
-       | pright =>
-         match d with
-         | dright d' => Success d'
-         | dleft _ => RecoverableError
-         | _ => TerminalError 
-         end
-       end.
-
-  End eval.
-
-  (** an alternative version of the compiler that keeps debug information. 
-     Theorem interp_debug_correct ensures that this version is kept in sync
-     with the simpler compiler.  This forces some code duplication, but the interpreter is relatively small and simple.  Trying to avoid code duplication complicates the (relatively longer) compilers and proofs. *)
-  Section eval_debug.
-
-  Inductive presult_debug A :=
-  | TerminalError_debug (s:string) (loc:camp_src_path) : presult_debug A
-  | RecoverableError_debug (s:string) : presult_debug A
-  | Success_debug (res:A) : presult_debug A.
-
-    (* begin hide *)
-  Arguments TerminalError_debug {A} s loc.
-  Arguments RecoverableError_debug {A} s.
-  Arguments Success_debug {A} res.
-  (* end hide *)
-
-  (* Not a ToString instance since it requires the top level pattern *)  
-  Definition print_presult_debug {A} {tos:ToString A} (p:camp) (pr:presult_debug A)
-    := match pr with
-         | TerminalError_debug s loc => "TerminalError: " ++ s ++ ". This error occurred in the bracketed code: \n" ++ (toString_camp_with_path p (rev loc))
-         | RecoverableError_debug s => "RecoverableError: " ++ s
-         | Success_debug res => "Success: " ++ toString res
-       end.
-
-  (** Useful lifting functions used in the evaluation of patterns. Used to handle the various possible presults *)
-  Definition liftpr_debug {A B:Type} (f:A->B) (pr:presult_debug A) : presult_debug B
-    := match pr with
-       | TerminalError_debug s loc => TerminalError_debug s loc
-       | RecoverableError_debug s => RecoverableError_debug s
-       | Success_debug a => Success_debug (f a)
-       end.
-
-  Definition bindpr_debug {A B:Type} (pr:presult_debug A) (f:A->presult_debug B) : presult_debug B
-    := match pr with
-       | TerminalError_debug s loc => TerminalError_debug s loc
-       | RecoverableError_debug s => RecoverableError_debug s
-       | Success_debug a => (f a)
-       end.
-
-  Lemma liftpr_debug_bindpr_debug {A B:Type} (f:A->B) pr :
-    liftpr_debug f pr = bindpr_debug pr (fun x => Success_debug (f x)).
-  Proof.
-    destruct pr; simpl; trivial.
-  Qed.
-
-  Fixpoint gather_successes_debug {A:Type} (os:list (presult_debug A)) : presult_debug (list A)
-    := match os with
-       | nil => Success_debug nil
-       | (TerminalError_debug s loc)::xs => TerminalError_debug s loc
-       | (RecoverableError_debug s)::xs => gather_successes_debug xs
-       | (Success_debug a)::xs => liftpr_debug (cons a) (gather_successes_debug xs)
-       end.
-
-  Fixpoint enforce_successes_debug {A:Type} (os:list (presult_debug A)) : presult_debug (list A)
-    := match os with
-       | nil => Success_debug nil
-       | (TerminalError_debug s loc)::xs => TerminalError_debug s loc
-       | (RecoverableError_debug s)::xs => RecoverableError_debug s
-       | (Success_debug a)::xs => liftpr_debug (cons a) (gather_successes_debug xs)
-       end.
-  
-  Definition op2tpr_debug {A:Type} (err:string) (loc:camp_src_path) (o:option A) : presult_debug A
-    := match o with
-       | None => TerminalError_debug err loc
-       | Some x => Success_debug x
-       end.
     
-  (* begin hide *)
-  Definition op2rpr_debug {A:Type} (err:string) (o:option A) : presult_debug A
-    := match o with
-       | None => RecoverableError_debug err
-       | Some x => Success_debug x
-       end.
-
-  Definition pr2op_debug (o:presult_debug data) : option data
-    := match o with
-       | RecoverableError_debug err => None
-       | TerminalError_debug _ _ => Some dunit
-       | Success_debug x => Some x
-       end.
-
-  (* end hide *)
-
-  (** Semantics of CAMP pattern, returning a presult *)
-  Context (h:brand_relation_t).
-  Context (constant_env:list(string*data)).
-
-  Context (print_env:bool).
+  (** * Traced Evaluation *)
   
-  Definition mk_err (desc:string) (p:camp) (bind:bindings) (it:data)
-    := toString p ++ " failed" ++ desc ++ "." ++
-                (if print_env
-                 then "\n Current environment (env): "
-                        ++ toString (drec bind)
-                 else "") ++
-                "\n Current scrutinee (it): "
-                ++ toString it ++
-                "\n".
+  (** An alternative version of the compiler that keeps debug
+     information. While this forces some code duplication, this is
+     mitigated by the fact that the evaluation code is relatively
+     small and simple. *)
+
+  (** The context is the same as for default evaluation, with an
+  additional printing flag. *)
+
+  Section EvaluationDebug.
+    Context (h:brand_relation_t).
+    Context (constant_env:list(string*data)).
+    Context (print_env:bool).
+
+    (** The following functions are used to produce error messages. *)
+    
+    Definition mk_err (desc:string) (p:camp) (bind:bindings) (it:data)
+      := toString p ++ " failed" ++ desc ++ "." ++
+                  (if print_env
+                   then "\n Current environment (env): "
+                          ++ toString (drec bind)
+                   else "") ++
+                  "\n Current scrutinee (it): "
+                  ++ toString it ++
+                  "\n".
   
-  (* It is important to separate out the debug messages.
+    (* It is important to separate out the debug messages.
      Otherwise, they get reduced by proofs, which is painful *)
-  Definition punop_err (p:camp) (bind:bindings) (it:data) (d:data) : string
-    := (mk_err "" p bind it ++ " The operator's argument was: " ++ toString d ++ "\n").
+    Definition punop_err (p:camp) (bind:bindings) (it:data) (d:data) : string
+      := (mk_err "" p bind it ++ " The operator's argument was: " ++ toString d ++ "\n").
+    
+    Definition binop_err (p:camp) (bind:bindings) (it:data) (d'₁ d'₂:data) : string
+      := (mk_err "" p bind it ++ " The operator's first argument was: " ++ toString d'₁
+                 ++ "\n The operator's second argument was: " ++ toString d'₂
+                 ++ "\n").
 
-  Definition binop_err (p:camp) (bind:bindings) (it:data) (d'₁ d'₂:data) : string
-    := (mk_err "" p bind it ++ " The operator's first argument was: " ++ toString d'₁
-               ++ "\n The operator's second argument was: " ++ toString d'₂
-       ++ "\n").
+    Definition pmap_err (p:camp) (bind:bindings) (it:data) : string
+      := mk_err " because the scrutinee was not a collection" p bind it.
 
-  Definition pmap_err (p:camp) (bind:bindings) (it:data) : string
-    := mk_err " because the scrutinee was not a collection" p bind it.
+    Definition passert_err (p:camp) (bind:bindings) (it d:data) : string
+      := mk_err " because the argument was not a boolean" p bind it
+                ++ " The argument to passert was: " ++ toString d
+                ++ "\n".
+    
+    Definition pletEnv_err (p:camp) (bind:bindings) (it d:data) : string
+      := mk_err " because its first argument was not a record" p bind it
+                ++ " The first argument to pletEnv was: " ++ toString d.
 
-  Definition passert_err (p:camp) (bind:bindings) (it d:data) : string
-    := mk_err " because the argument was not a boolean" p bind it
-              ++ " The argument to passert was: " ++ toString d
-               ++ "\n".
-
-  Definition pletEnv_err (p:camp) (bind:bindings) (it d:data) : string
-    := mk_err " because its first argument was not a record" p bind it
-              ++ " The first argument to pletEnv was: " ++ toString d.
-
-  Definition pleft_err (bind:bindings) (it:data) : string
-    := mk_err " because the scrutinee was an incompatible type" pleft bind it.
-
-  Definition pright_err (bind:bindings) (it:data) : string
+    Definition pleft_err (bind:bindings) (it:data) : string
+      := mk_err " because the scrutinee was an incompatible type" pleft bind it.
+    
+    Definition pright_err (bind:bindings) (it:data) : string
       := mk_err " because the scrutinee was an incompatible type" pright bind it.
-
-    Definition pgetconstant_err s (bind:bindings) (it:data) : string
+    
+    Definition pgetConstant_err s (bind:bindings) (it:data) : string
       := mk_err (" because the given field (" ++ s ++
-                ") is not a valid constant") (pgetconstant s) bind it
+                                              ") is not a valid constant") (pgetConstant s) bind it
                 ++ " The set of constants for this execution is: " ++
                 (bracketString "{" (joinStrings "; " (domain constant_env)) "}")
                 ++ "\n".
 
-  Fixpoint interp_debug (loc:camp_src_path) (p:camp) (bind:bindings) (d:data) : presult_debug data
-    := match p with
-       | pconst d' => Success_debug (normalize_data h d')
-       | punop op p₁ =>
-         match interp_debug (0::loc) p₁ bind d with
+    (** The alternative traced evaluation is defined as follows. *)
+    
+    Fixpoint camp_eval_debug (loc:camp_src_path) (p:camp) (bind:bindings) (d:data) : presult_debug data
+      := match p with
+         | pconst d' => Success_debug (normalize_data h d')
+         | punop op p₁ =>
+           match camp_eval_debug (0::loc) p₁ bind d with
            | TerminalError_debug s loc' => TerminalError_debug s loc'
            | RecoverableError_debug s => RecoverableError_debug s
            | Success_debug d' => 
              match fun_of_unaryop h op d' with
-               | None => TerminalError_debug (punop_err (punop op p₁) bind d d')  loc
-               | Some x => Success_debug x
+             | None => TerminalError_debug (punop_err (punop op p₁) bind d d')  loc
+             | Some x => Success_debug x
              end
-         end
-       | pbinop op p₁ p₂ =>
-         match interp_debug (0::loc) p₁ bind d with
+           end
+         | pbinop op p₁ p₂ =>
+           match camp_eval_debug (0::loc) p₁ bind d with
            | TerminalError_debug s loc' => TerminalError_debug s loc'
            | RecoverableError_debug s => RecoverableError_debug s
            | Success_debug d'₁ =>
-             match interp_debug (1::loc) p₂ bind d with
-               | TerminalError_debug s loc' => TerminalError_debug s loc'
-               | RecoverableError_debug s => RecoverableError_debug s
-               | Success_debug d'₂ =>
-                 match fun_of_binop h op d'₁ d'₂ with
-                   | None => TerminalError_debug (binop_err (pbinop op p₁ p₂) bind d d'₁ d'₂)  loc
-                   | Some x => Success_debug x
-                 end
+             match camp_eval_debug (1::loc) p₂ bind d with
+             | TerminalError_debug s loc' => TerminalError_debug s loc'
+             | RecoverableError_debug s => RecoverableError_debug s
+             | Success_debug d'₂ =>
+               match fun_of_binop h op d'₁ d'₂ with
+               | None => TerminalError_debug (binop_err (pbinop op p₁ p₂) bind d d'₁ d'₂)  loc
+               | Some x => Success_debug x
+               end
              end
-         end
-       | pmap p₁ =>
-         match d with
-         | dcoll l => liftpr_debug dcoll (gather_successes_debug (map (interp_debug (0::loc) p₁ bind) l))
-         | _ => TerminalError_debug (pmap_err (pmap p₁) bind d) loc
-
-         end
-(* Adds some unexpected complexity since the pattern used to calculate the key may return match failure.
-   How should we handle it? One option is to turn match failure into dunit, which possibly pushes part of the complexity
-   down to the algebra. Not sure what the other
-   options are ... - J
-       | pgroupBy p₁ =>
-         match d with
-         | dcoll l => op2tpr "groupBy failed"
-                             (lift dcoll
-                                   (group_by_nested_eval_kv (fun x => pr2op (interp_debug p₁ bind x)) l))
-         | _ => TerminalError_debug "pgroupBy evaluated when scrutinee is not a collection"
-         end *)
-       | passert p₁ =>
-         match interp_debug (0::loc) p₁ bind d with
+           end
+         | pmap p₁ =>
+           match d with
+           | dcoll l => liftpr_debug dcoll (gather_successes_debug (map (camp_eval_debug (0::loc) p₁ bind) l))
+           | _ => TerminalError_debug (pmap_err (pmap p₁) bind d) loc
+           end
+         | passert p₁ =>
+           match camp_eval_debug (0::loc) p₁ bind d with
            | TerminalError_debug s loc' => TerminalError_debug s loc'
            | RecoverableError_debug s => RecoverableError_debug s
            | Success_debug d' =>
              match d' with
-               | dbool true => Success_debug (drec nil)
-               | dbool false => RecoverableError_debug "assertion failure"
-               | _ => TerminalError_debug (passert_err (passert p₁) bind d d') loc
+             | dbool true => Success_debug (drec nil)
+             | dbool false => RecoverableError_debug "assertion failure"
+             | _ => TerminalError_debug (passert_err (passert p₁) bind d d') loc
              end
-         end
-       | porElse p₁ p₂ =>
-         match interp_debug (0::loc) p₁ bind d with
-         | TerminalError_debug s loc' => TerminalError_debug s loc'
-         | RecoverableError_debug _ => interp_debug (1::loc) p₂ bind d
-         | Success_debug x => Success_debug x
-         end
-       | pit => Success_debug d
-       | pletIt p₁ p₂ =>
-         match interp_debug (0::loc) p₁ bind d with
-         | TerminalError_debug s loc' => TerminalError_debug s loc'
-         | RecoverableError_debug s => RecoverableError_debug s
-         | Success_debug x => interp_debug (1::loc) p₂ bind x
-         end
-       | pgetconstant s =>
-         match edot constant_env s with
+           end
+         | porElse p₁ p₂ =>
+           match camp_eval_debug (0::loc) p₁ bind d with
+           | TerminalError_debug s loc' => TerminalError_debug s loc'
+           | RecoverableError_debug _ => camp_eval_debug (1::loc) p₂ bind d
+           | Success_debug x => Success_debug x
+           end
+         | pit => Success_debug d
+         | pletIt p₁ p₂ =>
+           match camp_eval_debug (0::loc) p₁ bind d with
+           | TerminalError_debug s loc' => TerminalError_debug s loc'
+           | RecoverableError_debug s => RecoverableError_debug s
+           | Success_debug x => camp_eval_debug (1::loc) p₂ bind x
+           end
+         | pgetConstant s =>
+           match edot constant_env s with
            | Some x => Success_debug x
-           | None => TerminalError_debug (pgetconstant_err s bind d) loc
-         end
-       | penv => Success_debug (drec bind)
-       | pletEnv p₁ p₂ =>
-         match interp_debug (0::loc) p₁ bind d with
+           | None => TerminalError_debug (pgetConstant_err s bind d) loc
+           end
+         | penv => Success_debug (drec bind)
+         | pletEnv p₁ p₂ =>
+           match camp_eval_debug (0::loc) p₁ bind d with
            | TerminalError_debug s loc' => TerminalError_debug s loc'
            | RecoverableError_debug s => RecoverableError_debug s
            | Success_debug rd'₁ => 
              match rd'₁ with
-               | drec d'₁ => match merge_bindings bind d'₁ with
-                               | Some bind' => interp_debug (1::loc) p₂ bind' d
-                               | None => RecoverableError_debug "bindings could not be unfied"
-                             end
-               | _ => TerminalError_debug (pletEnv_err (pletEnv p₁ p₂) bind d rd'₁) loc
+             | drec d'₁ => match merge_bindings bind d'₁ with
+                           | Some bind' => camp_eval_debug (1::loc) p₂ bind' d
+                           | None => RecoverableError_debug "bindings could not be unfied"
+                           end
+             | _ => TerminalError_debug (pletEnv_err (pletEnv p₁ p₂) bind d rd'₁) loc
              end
-         end
-       | pleft =>
-         match d with
-         | dleft d' => Success_debug d'
-         | dright _ => RecoverableError_debug "pleft called on a pright"
-         | _ => TerminalError_debug (pleft_err bind d) loc
-         end
-       | pright =>
-         match d with
-         | dright d' => Success_debug d'
-         | dleft _ => RecoverableError_debug "pright called on a pleft"
-         | _ => TerminalError_debug (pright_err bind d) loc
-         end
-       end.
+           end
+         | pleft =>
+           match d with
+           | dleft d' => Success_debug d'
+           | dright _ => RecoverableError_debug "pleft called on a pright"
+           | _ => TerminalError_debug (pleft_err bind d) loc
+           end
+         | pright =>
+           match d with
+           | dright d' => Success_debug d'
+           | dleft _ => RecoverableError_debug "pright called on a pleft"
+           | _ => TerminalError_debug (pright_err bind d) loc
+           end
+         end.
 
-      (* begin hide *)
-  Arguments TerminalError {A}.
-  Arguments RecoverableError {A}.
-  Arguments Success {A} res.
-  Arguments TerminalError_debug {A} s loc.
-  Arguments RecoverableError_debug {A} s.
-  Arguments Success_debug {A} res.
-  (* end hide *)
+    (** The following theorem states that traced evaluation is equivalent to regular evaluation. *)
+    
+    Theorem camp_eval_debug_correct (loc:camp_src_path) (p:camp) (bind:bindings) (d:data) :
+      presult_same
+        (camp_eval h constant_env p bind d)
+        (camp_eval_debug loc p bind d).
+    Proof.
+      revert loc bind d.
+      camp_cases (induction p) Case; simpl; intros.
+      - trivial.
+      - apply bindpr_presult_same; [eauto | ]; intros.
+        destruct (fun_of_unaryop h u x); simpl; trivial. 
+      - apply bindpr_presult_same; [eauto | ]; intros.
+        apply bindpr_presult_same; [eauto | ]; intros.
+        destruct (fun_of_binop h b x x0); simpl; trivial.
+      - destruct d; simpl; trivial.
+        apply liftpr_presult_same.
+        apply gather_successes_presult_same.
+        rewrite <- Forall2_map.
+        apply Forall2_refl; red; intros.
+        apply IHp.
+      - apply bindpr_presult_same; [eauto | ]; intros.
+        destruct x; simpl; trivial.
+        destruct b; simpl; trivial.
+      - specialize (IHp1 (0::loc) bind d); red in IHp1.
+        repeat match_destr_in IHp1; try tauto.
+      - trivial.
+      - apply bindpr_presult_same; [eauto | ]; intros.
+        eauto.
+      - unfold op2tpr. match_destr; simpl; trivial.
+      - trivial.
+      - apply bindpr_presult_same; [eauto | ]; intros.
+        destruct x; simpl; trivial.
+        destruct (merge_bindings bind l); simpl; trivial.
+      - destruct d; simpl; trivial.
+      - destruct d; simpl; trivial.
+    Qed.
 
-  Definition presult_same {A} (res:presult A) (res_debug:presult_debug A) :=
-    match res, res_debug with
-      | TerminalError, TerminalError_debug _ _ => True
-      | RecoverableError, RecoverableError_debug _ => True
-      | Success x, Success_debug y => x = y
-      | _, _ => False
-    end.
+  End EvaluationDebug.
 
-  Lemma liftpr_presult_same {A B} (f:A->B) d1 d2 :
-      presult_same d1 d2 ->
-      presult_same (liftpr f d1) (liftpr_debug f d2).
-  Proof.
-    unfold presult_same.
-    destruct d1; destruct d2; simpl; congruence.
-  Qed.
+  (** * Toplevel *)
+  
+  (** Top-level evaluation functions are used externally by the Q*cert
+  compiler. They take a CAMP pattern and a global environment as
+  input. The initial local environment is set to an empty record, and
+  the initial current value to unit. *)
 
-  Lemma gather_successes_presult_same {A} d1 d2 :
-      Forall2 (@presult_same A) d1 d2 ->
-      presult_same (gather_successes d1) (gather_successes_debug d2).
-  Proof.
-    unfold presult_same.
-    induction 1; simpl; trivial.
-    destruct x; destruct y; destruct (gather_successes l); destruct (gather_successes_debug l'); simpl in *; subst; intuition.
-  Qed.
-
-  Lemma bindpr_presult_same {A B} d1 d2 f1 f2:
-    presult_same d1 d2 ->
-    (forall x, presult_same (f1 x) (f2 x)) ->
-    presult_same (@bindpr A B d1 f1) (bindpr_debug d2 f2).
-  Proof.
-    destruct d1; destruct d2; simpl in *; try tauto.
-    intros; subst; auto.
-  Qed.
-
-  Theorem interp_debug_correct (loc:camp_src_path) (p:camp) (bind:bindings) (d:data) :
-    presult_same
-      (interp h constant_env p bind d)
-      (interp_debug loc p bind d).
-  Proof.
-    revert loc bind d.
-    camp_cases (induction p) Case; simpl; intros.
-    - trivial.
-    - apply bindpr_presult_same; [eauto | ]; intros.
-      destruct (fun_of_unaryop h u x); simpl; trivial. 
-    - apply bindpr_presult_same; [eauto | ]; intros.
-      apply bindpr_presult_same; [eauto | ]; intros.
-      destruct (fun_of_binop h b x x0); simpl; trivial.
-    - destruct d; simpl; trivial.
-      apply liftpr_presult_same.
-      apply gather_successes_presult_same.
-      rewrite <- Forall2_map.
-      apply Forall2_refl; red; intros.
-      apply IHp.
-    - apply bindpr_presult_same; [eauto | ]; intros.
-      destruct x; simpl; trivial.
-      destruct b; simpl; trivial.
-    - specialize (IHp1 (0::loc) bind d); red in IHp1.
-      repeat match_destr_in IHp1; try tauto.
-    - trivial.
-    - apply bindpr_presult_same; [eauto | ]; intros.
-      eauto.
-    - unfold op2tpr. match_destr; simpl; trivial.
-    - trivial.
-    - apply bindpr_presult_same; [eauto | ]; intros.
-      destruct x; simpl; trivial.
-      destruct (merge_bindings bind l); simpl; trivial.
-    - destruct d; simpl; trivial.
-    - destruct d; simpl; trivial.
-  Qed.
-
-  End eval_debug.
-
-  Lemma interp_const_sort h c p b d:
-    interp h (rec_sort c) p b d = interp h c p b d.
-  Proof.
-    revert c b d.
-    induction p; simpl; unfold olift, olift2; intros; trivial;
-    try rewrite IHp; try rewrite IHp1; try rewrite IHp2; trivial.
-    - match_destr.
-      f_equal.
-      f_equal.
-      apply map_ext; intros.
-      auto.
-    - unfold bindpr.
-      match_destr.
-    - unfold edot.
-      rewrite assoc_lookupr_drec_sort.
-      trivial.
-    - unfold bindpr. match_destr.
-      destruct res; trivial.
-      match_destr.
-  Qed.
-
-  (** Semantics of CAMP patterns, returning a presult *)
-  Definition eval_pattern_debug (h:list(string*string)) (print_env:bool) (p:camp) (world:list data)
-    : presult_debug data
-    := interp_debug h (mkWorld world) print_env nil p nil dunit.
-
-  Definition eval_pattern_res_to_string
-             (h:list(string*string)) (print_env:bool) (p:camp) (world:list data)
-    : string
-    := print_presult_debug p
-                           (interp_debug h
-                                         (mkWorld world)
-                                         print_env nil p nil dunit).
-
-  Definition eval_pattern_res (h:list(string*string)) (p:camp) (world:list data)
-    : presult data
-    := interp h (mkWorld world) p nil dunit.
-
-  Definition eval_pattern (h:list(string*string)) (p:camp) (world:list data)
-    : option (list data)
-    := match eval_pattern_res h p world with
-       | Success _ l => Some (l::nil)
-       | RecoverableError _ => Some nil
-       | TerminalError _ => None
-       end.
-
+  (** The result of evaluation is lifted back from presult to and
+  optional value for consistency with evaluation functions for the
+  other intermediate languages. *)
+  
   Section Top.
     Context (h:brand_relation_t).
 
-    Definition camp_eval_top (q:camp) (cenv:bindings) :=
-      match interp h (rec_sort cenv) q nil dunit with
-      | Success _ l => Some (dcoll (l::nil))
-      | RecoverableError _ => Some (dcoll nil)
-      | TerminalError _ => None
+    Definition presult_to_result (pr:presult data) : option data :=
+      match pr with
+      | Success l => Some (dcoll (l::nil))
+      | RecoverableError => Some (dcoll nil)
+      | TerminalError => None
       end.
+
+    Definition camp_eval_top_to_presult (q:camp) (global_env:bindings) : presult data :=
+      camp_eval h (rec_sort global_env) q nil dunit.
+
+    (** The main top-level evaluation function for CAMP is as follows. *)
+    
+    Definition camp_eval_top (q:camp) (global_env:bindings) : option data :=
+      presult_to_result (camp_eval_top_to_presult q global_env).
+
+    Definition presult_debug_to_result (pr:presult_debug data) : option data :=
+      match pr with
+      | Success_debug l => Some (dcoll (l::nil))
+      | RecoverableError_debug _ => Some (dcoll nil)
+      | TerminalError_debug _ _ => None
+      end.
+
+    Definition camp_eval_top_debug_to_presult_debug
+               (debug:bool) (q:camp) (global_env:bindings) : presult_debug data :=
+      camp_eval_debug h (rec_sort global_env) debug nil q nil dunit.
+
+    Theorem camp_eval_top_debug_correct (debug:bool) (p:camp) (global_env:bindings) (d:data) :
+      presult_same
+        (camp_eval_top_to_presult p global_env)
+        (camp_eval_top_debug_to_presult_debug debug p global_env).
+    Proof.
+      unfold camp_eval_top_to_presult.
+      unfold camp_eval_top_debug_to_presult_debug.
+      apply camp_eval_debug_correct.
+    Qed.
+    
+    Definition camp_eval_top_debug_to_data
+               (debug:bool) (q:camp) (global_env:bindings) : option data :=
+      presult_debug_to_result (camp_eval_debug h (rec_sort global_env) debug nil q nil dunit).
+
+    (** The main top-level traced evaluation function for CAMP is as follows. *)
+    
+    Definition camp_eval_top_debug (debug:bool) (q:camp) (global_env:bindings) : string :=
+      print_presult_debug q toString_camp_with_path
+                          (camp_eval_top_debug_to_presult_debug debug q global_env).
   End Top.
+
 End CAMP.
 
 (* begin hide *)
-Arguments TerminalError {A}.
-Arguments RecoverableError {A}.
-Arguments Success {A} res.
-
 Tactic Notation "camp_cases" tactic(first) ident(c) :=
   first;
   [ Case_aux c "pconst"%string
   | Case_aux c "punop"%string
   | Case_aux c "pbinop"%string
   | Case_aux c "pmap"%string
-(*| Case_aux c "pgroupBy"%string *)
   | Case_aux c "passert"%string
   | Case_aux c "porElse"%string
   | Case_aux c "pit"%string
   | Case_aux c "pletIt"%string
-  | Case_aux c "pgetconstant"%string
+  | Case_aux c "pgetConstant"%string
   | Case_aux c "penv"%string
   | Case_aux c "pletEnv"%string
   | Case_aux c "pleft"%string
