coq/CAMP/Lang/CAMPUtil.v
@@ -1,0 +1,251 @@
+(*
+ * Copyright 2015-2016 IBM Corporation
+ *
+ * Licensed under the Apache License, Version 2.0 (the "License");
+ * you may not use this file except in compliance with the License.
+ * You may obtain a copy of the License at
+ *
+ * http://www.apache.org/licenses/LICENSE-2.0
+ *
+ * Unless required by applicable law or agreed to in writing, software
+ * distributed under the License is distributed on an "AS IS" BASIS,
+ * WITHOUT WARRANTIES OR CONDITIONS OF ANY KIND, either express or implied.
+ * See the License for the specific language governing permissions and
+ * limitations under the License.
+ *)
+
+(** Encoding and utility functions to support the result of evaluation
+over CAMP patterns. *)
+
+Section CAMPUtil.
+
+  Require Import String.
+  Require Import List.
+  Require Import EquivDec.
+  Require Import Morphisms.
+  Require Import BasicRuntime.
+  Local Open Scope string.
+
+  (** Evaluating a CAMP pattern returns a presult, which includes two
+  kinds of errors: either a match failure, which is recoverable, or a
+  terminal error. *)
+  
+  Inductive presult A :=
+  | TerminalError : presult A
+  | RecoverableError : presult A
+  | Success (res:A) : presult A.
+
+  (* begin hide *)
+  Arguments TerminalError {A}.
+  Arguments RecoverableError {A}.
+  Arguments Success {A} res.
+  (* end hide *)
+
+  (** Equality between two presult is decidable *)
+  
+  Global Instance presult_eqdec {A} {dec:EqDec A eq} :
+    EqDec (presult A) eq.
+  Proof.
+    red; unfold equiv, complement.
+    destruct x; destruct y; simpl;
+      try solve [right; inversion 1]; eauto 2.
+    destruct (res == res0); unfold equiv, complement in *;
+      [left | right; inversion 1]; congruence.
+  Defined.
+  
+  (** Prints a presult *)
+  
+  Global Instance print_presult {A} {tos:ToString A} : ToString (presult A)
+    := { toString :=
+           fun pr =>
+             match pr with
+             | TerminalError => "TerminalError (for more info, use debug mode)"
+             | RecoverableError => "RecoverableError (for more info, use debug mode)"
+             | Success res => "Success: " ++ toString res
+             end
+       }.
+  
+  (** Lifting functions used in the evaluation of patterns. Used to handle the various possible presults during evaluation. *)
+  Definition liftpr {A B:Type} (f:A->B) (pr:presult A) : presult B
+    := match pr with
+       | TerminalError => TerminalError
+       | RecoverableError => RecoverableError
+       | Success a => Success (f a)
+       end.
+
+  Definition bindpr {A B:Type} (pr:presult A) (f:A->presult B) : presult B
+    := match pr with
+       | TerminalError => TerminalError 
+       | RecoverableError => RecoverableError
+       | Success a => (f a)
+       end.
+
+  Lemma liftpr_bindpr {A B:Type} (f:A->B) pr :
+    liftpr f pr = bindpr pr (fun x => Success (f x)).
+  Proof.
+    destruct pr; simpl; trivial.
+  Qed.
+
+  (** Accumulates successful evaluation, skipping match failures. A terminal error is always final. *)
+  
+  Fixpoint gather_successes {A:Type} (os:list (presult A)) : presult (list A)
+    := match os with
+       | nil => Success nil
+       | (TerminalError)::xs => TerminalError 
+       | (RecoverableError)::xs => gather_successes xs
+       | (Success a)::xs => liftpr (cons a) (gather_successes xs)
+       end.
+
+  (** Accumulates successful evaluation, but propagating match failure to the top *)
+  
+  Fixpoint enforce_successes {A:Type} (os:list (presult A)) : presult (list A)
+    := match os with
+       | nil => Success nil
+       | (TerminalError)::xs => TerminalError
+       | (RecoverableError)::xs => RecoverableError
+       | (Success a)::xs => liftpr (cons a) (gather_successes xs)
+       end.
+  
+  Definition op2tpr {A:Type} (o:option A) : presult A
+    := match o with
+       | None => TerminalError
+       | Some x => Success x
+       end.
+
+  Definition op2rpr {A:Type} (o:option A) : presult A
+    := match o with
+       | None => RecoverableError
+       | Some x => Success x
+       end.
+
+  Section Debug.
+  (* If we were reasoning about this formally, we would want to use a proper
+     one-hole context.  Since we are not, a trail of choices suffices *)
+  Definition camp_src_path
+    := list nat.
+
+    Inductive presult_debug A :=
+    | TerminalError_debug (s:string) (loc:camp_src_path) : presult_debug A
+    | RecoverableError_debug (s:string) : presult_debug A
+    | Success_debug (res:A) : presult_debug A.
+
+    (* begin hide *)
+    Arguments TerminalError_debug {A} s loc.
+    Arguments RecoverableError_debug {A} s.
+    Arguments Success_debug {A} res.
+    (* end hide *)
+
+    (* Not a ToString instance since it requires the top level pattern *)  
+    Definition print_presult_debug {A} {B} {tos:ToString A} (p:B)
+               (pPrint:B -> camp_src_path -> string) (pr:presult_debug A)
+      := match pr with
+         | TerminalError_debug s loc => "TerminalError: " ++ s ++ ". This error occurred in the bracketed code: \n" ++ (pPrint p (rev loc))
+         | RecoverableError_debug s => "RecoverableError: " ++ s
+         | Success_debug res => "Success: " ++ toString res
+         end.
+    
+    (** Useful lifting functions used in the evaluation of patterns. Used to handle the various possible presults *)
+    Definition liftpr_debug {A B:Type} (f:A->B) (pr:presult_debug A) : presult_debug B
+      := match pr with
+         | TerminalError_debug s loc => TerminalError_debug s loc
+         | RecoverableError_debug s => RecoverableError_debug s
+         | Success_debug a => Success_debug (f a)
+         end.
+
+    Definition bindpr_debug {A B:Type} (pr:presult_debug A) (f:A->presult_debug B) : presult_debug B
+      := match pr with
+         | TerminalError_debug s loc => TerminalError_debug s loc
+         | RecoverableError_debug s => RecoverableError_debug s
+         | Success_debug a => (f a)
+         end.
+
+    Lemma liftpr_debug_bindpr_debug {A B:Type} (f:A->B) pr :
+      liftpr_debug f pr = bindpr_debug pr (fun x => Success_debug (f x)).
+    Proof.
+      destruct pr; simpl; trivial.
+    Qed.
+
+    Fixpoint gather_successes_debug {A:Type} (os:list (presult_debug A)) : presult_debug (list A)
+      := match os with
+         | nil => Success_debug nil
+         | (TerminalError_debug s loc)::xs => TerminalError_debug s loc
+         | (RecoverableError_debug s)::xs => gather_successes_debug xs
+         | (Success_debug a)::xs => liftpr_debug (cons a) (gather_successes_debug xs)
+         end.
+
+    Fixpoint enforce_successes_debug {A:Type} (os:list (presult_debug A)) : presult_debug (list A)
+      := match os with
+         | nil => Success_debug nil
+         | (TerminalError_debug s loc)::xs => TerminalError_debug s loc
+         | (RecoverableError_debug s)::xs => RecoverableError_debug s
+         | (Success_debug a)::xs => liftpr_debug (cons a) (gather_successes_debug xs)
+         end.
+  
+    Definition op2tpr_debug {A:Type} (err:string) (loc:camp_src_path) (o:option A) : presult_debug A
+      := match o with
+         | None => TerminalError_debug err loc
+         | Some x => Success_debug x
+         end.
+    
+    Definition op2rpr_debug {A:Type} (err:string) (o:option A) : presult_debug A
+      := match o with
+         | None => RecoverableError_debug err
+         | Some x => Success_debug x
+         end.
+
+    Definition presult_same {A} (res:presult A) (res_debug:presult_debug A) :=
+      match res, res_debug with
+      | TerminalError, TerminalError_debug _ _ => True
+      | RecoverableError, RecoverableError_debug _ => True
+      | Success x, Success_debug y => x = y
+      | _, _ => False
+      end.
+    
+    Lemma liftpr_presult_same {A B} (f:A->B) d1 d2 :
+      presult_same d1 d2 ->
+      presult_same (liftpr f d1) (liftpr_debug f d2).
+    Proof.
+      unfold presult_same.
+      destruct d1; destruct d2; simpl; congruence.
+    Qed.
+
+    Lemma gather_successes_presult_same {A} d1 d2 :
+      Forall2 (@presult_same A) d1 d2 ->
+      presult_same (gather_successes d1) (gather_successes_debug d2).
+    Proof.
+      unfold presult_same.
+      induction 1; simpl; trivial.
+      destruct x; destruct y; destruct (gather_successes l); destruct (gather_successes_debug l'); simpl in *; subst; intuition.
+    Qed.
+    
+    Lemma bindpr_presult_same {A B} d1 d2 f1 f2:
+      presult_same d1 d2 ->
+      (forall x, presult_same (f1 x) (f2 x)) ->
+      presult_same (@bindpr A B d1 f1) (bindpr_debug d2 f2).
+    Proof.
+      destruct d1; destruct d2; simpl in *; try tauto.
+      intros; subst; auto.
+    Qed.
+    
+  End Debug.
+
+End CAMPUtil.
+
+(* begin hide *)
+Arguments TerminalError {A}.
+Arguments RecoverableError {A}.
+Arguments Success {A} res.
+
+Arguments TerminalError {A}.
+Arguments RecoverableError {A}.
+Arguments Success {A} res.
+Arguments TerminalError_debug {A} s loc.
+Arguments RecoverableError_debug {A} s.
+Arguments Success_debug {A} res.
+(* end hide *)
+
+(* 
+*** Local Variables: ***
+*** coq-load-path: (("../../../coq" "Qcert")) ***
+*** End: ***
+*)
