scripts/gather_glob.sh
@@ -1,0 +1,16 @@
+#!/bin/bash
+
+declare -a WHITELIST=(".glob")
+
+for FILE in "$@"
+do
+    for ending in "${WHITELIST[@]}"
+    do
+	BASE=${FILE%%${ending}}
+	if [[ "$FILE" == "$BASE$ending" ]]
+	then
+	    echo "copying glob $FILE"
+	    cp "${FILE}" docs/globs
+	fi
+    done
+done     
